src/riot/asn1/ASN1.Spec.Value.BigInteger.fsti
@@ -1,0 +1,64 @@
+module ASN1.Spec.Value.BigInteger
+
+open ASN1.Spec.Base
+open LowParse.Spec.SeqBytes.Base
+
+open ASN1.Base
+open ASN1.Spec.Tag
+open ASN1.Spec.Length
+
+open FStar.Integers
+
+module B32 = FStar.Bytes
+
+unfold
+let big_integer_as_octet_string_t
+= x: datatype_of_asn1_type OCTET_STRING
+  { let (.[]) = B32.index in
+    v (dfst x) > 0 /\                      // no nil
+    ( if (v (dfst x) > 1) then
+      ( (dsnd x).[0] =!= 0x00uy )  // no leading zero byte if length > 1
+      else ( True ) ) /\
+    ( if ((dsnd x).[0] >= 0x80uy) then   // leave one space for leading zero byte
+      ( v (dfst x) <= asn1_length_max - 7 )
+      else ( True ) ) }
+
+let asn1_value_length_of_big_integer
+= l: asn1_length_t { 1 <= l /\ l <= asn1_length_max - 6}
+
+unfold
+let valid_big_integer_as_octet_string_prop
+  (l: asn1_value_length_of_big_integer)
+  (x: big_integer_as_octet_string_t)
+: Type0
+= v (dfst x) > 0 /\
+  ( let (.[]) = B32.index in
+    if l = 1 then
+    ( v (dfst x) == l /\ (dsnd x).[0] < 0x80uy )
+    else if ((dsnd x).[0] >= 0x80uy) then
+    ( v (dfst x) == l - 1 )
+    else
+    ( v (dfst x) == l /\ (dsnd x).[0] > 0x00uy ) )
+
+let parse_big_integer_as_octet_string_kind (l: asn1_value_length_of_big_integer) = constant_size_parser_kind l
+
+val parse_big_integer_as_octet_string
+  (l: asn1_value_length_of_big_integer)
+: parser (parse_big_integer_as_octet_string_kind l) (x: big_integer_as_octet_string_t {valid_big_integer_as_octet_string_prop l x})
+
+val serialize_big_integer_as_octet_string
+  (l: asn1_value_length_of_big_integer)
+: serializer (parse_big_integer_as_octet_string l)
+
+// val lemma_serialize_big_integer_as_octet_string_unfold
+//   (l: asn1_value_length_of_big_integer)
+//   (value: get_parser_type (parse_big_integer_as_octet_string l))
+// : Lemma (
+//   serialize (serialize_big_integer_as_octet_string l) value ==
+//   serialize (serialize_seq_flbytes l) (synth_big_integer_as_octet_string_inverse l value))
+
+val lemma_serialize_big_integer_as_octet_string_size
+  (l: asn1_value_length_of_big_integer)
+  (value: get_parser_type (parse_big_integer_as_octet_string l))
+: Lemma (
+  Seq.length (serialize (serialize_big_integer_as_octet_string l) value) == l)
